Source/DafnyCore/Resolver/ModuleResolver.cs
@@ -2489,10 +2489,7 @@ namespace Microsoft.Dafny {
           reporter.Error(MessageSource.Resolver, member.Origin,
             $"{traitMember.WhatKindAndName} is inherited from trait '{trait.Name}' and is not allowed to be re-declared");
         } else if (traitMember.TryCastToInvariant(Options, reporter, MessageSource.Resolver, out var invariant)) {
-          if (invariant.Body is not LiteralExpr { Value: true }) {
-            // TODO(somayyas) eventually implement overriding invariant
-            reporter.Error(MessageSource.Resolver, invariant.Origin, "overriding trait invariant is not yet supported");
-          }
+          reporter.Error(MessageSource.Resolver, invariant.Origin, "overriding the invariant of a trait is not supported");
         } else if ((traitMember as Function)?.Body != null || (traitMember as MethodOrConstructor)?.Body != null) {
           // the overridden member is a fully defined function or method, so the class is not allowed to do anything with it other than silently inherit it
           reporter.Error(MessageSource.Resolver, member.Origin,
