Source/DafnyCore/Rewriters/InvariantRewriter.cs
@@ -15,7 +15,8 @@ public class InvariantRewriter(Program program, ErrorReporter reporter) : IRewri
   
   // Add invariants as pre- and post-conditions
   void PreResolveTopLevelDecl(TopLevelDeclWithMembers cl) {
-    var invariantMember = (Invariant)cl.Members.Find(member => member is Invariant);
+    // Search for inherited invariants too! We must please the override checker
+    var invariantMember = cl.Invariant;
 
     if (invariantMember is null) {
       // No invariant, nothing to be done
@@ -28,6 +29,9 @@ public class InvariantRewriter(Program program, ErrorReporter reporter) : IRewri
     
     // We use the underlying invariant clauses instead of the predicate body
     // For proper error localization
+    // TODO(somayyas): kind of a gross and inconsistent way of preserving attributes,
+    // we should probably just call the invariant directly
+    
     var clauses = invariantMember.Clauses;
     foreach (var clause in clauses) {
       if (!Attributes.Contains(clause.Attributes, "error")) {
@@ -36,20 +40,22 @@ public class InvariantRewriter(Program program, ErrorReporter reporter) : IRewri
       }
     }
     
+    // Note: the following transformations approximate assuming/asserting the invariant for every object in the open set
+    // when it is just {this}. Once we have openness annotations, this will have to be generalized.
     foreach (var member in cl.Members) {
       switch (member) {
         case Constructor ctor: // Constructors have the invariant as additional ensures clauses
-          ctor.Ens.AddRange(clauses); // See below why invariant clauses are added last
+          ctor.Ens.InsertRange(0, clauses);
           break;
-        case Method method: // Currently, we assume that each method is public and, as such, needs to require/ensure the invariant
+        case Method { IsStatic: false } method: // Currently, we assume that each (instance) method is public and, as such, needs to require/ensure the invariant
           // Have to add the invariant at the front of the requires clauses, in case subsequent clauses depend on them to be well-formed
           method.Req.InsertRange(0, clauses);
-          method.Ens.AddRange(clauses); // Dually, the invariant is ensured last
+          method.Ens.InsertRange(0, clauses); // Postcondition may depend on invariant for well-formedness
           break;
         case Invariant:
-          break; // Nothing to do for invariants
-        case Function function: // Functions need only assume the invariant TODO: also hits functions that should be exempt
-          //xfunction.Req.InsertRange(0, clauses);
+          break; // Nothing to do for invariants (have to catch it before Function)
+        case Function function: // Functions need only assume the invariant
+          function.Req.InsertRange(0, clauses);
           break;
       }
     }
