Source/DafnyCore/Verifier/BoogieGenerator.cs
@@ -780,7 +780,16 @@ namespace Microsoft.Dafny {
         // conversion functions
         AddBitvectorNatConversionFunction(w);
       }
-
+      
+      if (options.Get(CommonOptionBag.CheckInvariants)) {
+        // revealed function $OpenHeapRelated($open: Set, $heap: Heap): bool
+        sink.AddTopLevelDeclaration(new Bpl.Function(Bpl.Token.NoToken, "$OpenHeapRelated", [],
+          [new Bpl.Formal(Token.NoToken, new(Bpl.Token.NoToken, "$open", Predef.SetType), true),
+           new Bpl.Formal(Token.NoToken, new(Bpl.Token.NoToken, "$heap", Predef.HeapType), true) ],
+           new Bpl.Formal(Token.NoToken, new(Bpl.Token.NoToken, "", Bpl.Type.Bool), false))
+        );
+      }
+      
       foreach (TopLevelDecl d in program.SystemModuleManager.SystemModule.TopLevelDecls) {
         CurrentDeclaration = d;
         if (d is AbstractTypeDecl abstractType) {
@@ -2128,6 +2137,29 @@ namespace Microsoft.Dafny {
         (t, e, d, q) => builder.Add(Assert(t, e, d, builder.Context, q)),
         (t, e) => builder.Add(TrAssumeCmd(t, e)),
         desc, kv);
+    }
+    
+    public Expr CheckFrameExcludes(IOrigin tok, List<FrameExpression> calleeFrame,
+      Expression receiverReplacement, Dictionary<IVariable, Expression /*!*/> substMap,
+      ExpressionTranslator /*!*/ etran, Boogie.Expr /*!*/ excluded) {
+      Contract.Requires(tok != null);
+      Contract.Requires(calleeFrame != null);
+      Contract.Requires(receiverReplacement == null || substMap != null);
+      Contract.Requires(etran != null);
+      Contract.Requires(Predef != null);
+
+      // emit: assert (forall o: ref, f: Field :: o != null && $Heap[o,alloc] && (o,f) in subFrame && o in $Open ==> o != excluded);
+      var oVar = new Bpl.BoundVariable(tok, new Bpl.TypedIdent(tok, "$o", Predef.RefType));
+      var o = new Bpl.IdentifierExpr(tok, oVar);
+      var fVar = new Bpl.BoundVariable(tok, new Bpl.TypedIdent(tok, "$f", Predef.FieldName(tok)));
+      var f = new Bpl.IdentifierExpr(tok, fVar);
+      var ante = Bpl.Expr.And(Bpl.Expr.Neq(o, Predef.Null), etran.IsAlloced(tok, o));
+      var oInCallee = InRWClause(tok, o, f, calleeFrame, etran, receiverReplacement, substMap);
+      var isExcluded = Bpl.Expr.Neq(o, excluded);
+      etran.OpenFormal(tok, out _, out var openExprDafny);
+      var q = new Bpl.ForallExpr(tok, [], [oVar, fVar],
+        BplImp(BplAnd([ante, oInCallee, etran.TrExpr(new BinaryExpr(tok, BinaryExpr.ResolvedOpcode.NotInSet, receiverReplacement, openExprDafny))]), isExcluded));
+      return q;
     }
 
     void CheckFrameSubset(IOrigin tok, List<FrameExpression> calleeFrame,
@@ -4142,8 +4174,15 @@ namespace Microsoft.Dafny {
       Contract.Requires(tok != null);
       Contract.Requires(etran != null);
       Contract.Ensures(Contract.Result<AssumeCmd>() != null);
+      
+      Expr expr = FunctionCall(tok, BuiltinFunction.IsGoodHeap, null, etran.HeapExpr);
+      
+      if (options.Get(CommonOptionBag.CheckInvariants)) {
+        etran.OpenFormal(tok, out var openExpr, out _);
+        expr = BplAnd(expr, FunctionCall(tok, BuiltinFunction.OpenHeapRelated, null, openExpr, etran.HeapExpr));
+      }
 
-      return TrAssumeCmd(tok, FunctionCall(tok, BuiltinFunction.IsGoodHeap, null, etran.HeapExpr));
+      return TrAssumeCmd(tok, expr);
     }
 
     /// <summary>
