Source/IntegrationTests/TestFiles/LitTests/LitTest/invariants/Counter.dfy
@@ -1,21 +1,32 @@
 // RUN: %verify --type-system-refresh --check-invariants "%s" > "%t"
 // RUN: %diff "%s.expect" "%t"
 
-// Store the old(value) since we don't yet have twostate invariants
+// Store the old(value) and since we don't yet have twostate invariants
+// The stuttering bit has the effect of taking the reflexive closure of the predicate
+//   value == old_value + 1
+// as if it were a relation on heaps, so that the invariant holds at the end of the constructor
 class Counter {
   ghost var old_value: nat
-  ghost var value: nat
+  var value: nat
+  var stuttering: bool
+  invariant stuttering || value == old_value + 1
   constructor() {
+    stuttering := true;
     old_value := 0;
     value     := 0;
   }
   method Increment()
     modifies this
-    ensures this.invariant()
   {
+    stuttering := false;
     old_value := value;
     value     := value + 1;
   }
-  invariant old_value == value || value == old_value + 1
 }
 
+lemma ReasonAboutCounter(c: Counter)
+  requires !c.stuttering
+  ensures c.value == c.old_value + 1
+{
+  assert c.invariant(); // kronk! fire the axiom!
+}
