Source/IntegrationTests/TestFiles/LitTests/LitTest/invariants/Account.dfy
@@ -1,0 +1,33 @@
+class Account {
+  var credit: nat
+  var debit: nat
+  // NB: can't use Balance() here b/c it would be recursive
+  invariant credit - debit >= 0
+  function Balance(): nat // NB: uses the invariant to be well-defined
+    reads this
+  {
+    credit - debit
+  }
+  method Withdraw(amount: nat)
+    requires Balance() - amount >= 0
+    ensures Balance() == old(Balance()) - amount // NB: this uses the invariant to be well-defined
+    modifies this
+  {
+    debit := debit + amount;
+  }
+  method Deposit(amount: nat)
+    ensures Balance() == old(Balance()) + amount
+    modifies this
+  {
+    credit := credit + amount;
+  }
+}
+
+method Use(a: Account)
+  modifies a
+{
+  a.Deposit(100) by { assert a.invariant(); } // need this for the following call to be well-formed
+  a.Withdraw(50);
+  a.Withdraw(50);
+  assert a.Balance() >= 0;
+}
