Source/IntegrationTests/TestFiles/LitTests/LitTest/invariants/DerivedInvariant.dfy
@@ -1,0 +1,31 @@
+trait Base {
+   var x: int
+   function FooSpec(): int
+     reads this
+   method Foo() returns (r: int)
+     ensures r == FooSpec()
+   //invariant x != 0 // ok, but subclasses cannot then declare an invariant
+}
+
+class Ext extends Base {
+  var y: int
+  invariant y != 0 // note: invariant can't refer to x
+  function FooSpec(): int
+    reads this
+  {
+    1 / y
+  }
+  method Foo() returns (r: int)
+    ensures r == FooSpec()
+  {
+    r := FooSpec();
+  }
+}
+
+method Upcast(e: Ext)
+  modifies e
+{
+  var b := e as Base;
+  b.x := 0; // no problem;
+  e.y := 1; // checks invariant, no problem
+}
