Source/IntegrationTests/TestFiles/LitTests/LitTest/invariants/TempInvariantBreaking.dfy
@@ -1,0 +1,37 @@
+class C {
+  var x: int
+  
+  invariant x != 0
+
+  constructor() {
+     x := 1; 
+     x := 0; // breaking the invariant here is fine
+     x := 1; // as long at it is satisfied at the end
+  }
+
+  method TemporarilyBreakInvariant()
+    modifies this
+  {
+     x := 0; // temporarily breaking the invariant outside the constructor is allowed
+     //UseInvariant(this); // error: invariant doesn't hold here (force checked, since this is open)
+     var me := this;
+     //UseInvariant(me); //  error: same as above (this can be copied as much as you want)
+     x := 1;
+  }
+ 
+  static method UseInvariant(c: C) 
+  {
+    var y := 3 / c.x by { assert c.invariant(); }
+  }
+
+  static method External(c: C)
+  {
+     UseInvariant(c);
+  }
+
+  static method External2(c: C)
+    modifies c
+  {
+     //c.x := 0; // verifier error: c's invariant cannot be re-established
+  }
+}
