Source/IntegrationTests/TestFiles/LitTests/LitTest/invariants/TwoPhaseConstructors.dfy
@@ -1,0 +1,27 @@
+class C {
+  var valid: bool
+  invariant valid
+
+  constructor SinglePhase() {
+    //assert valid; // error
+    valid := true;
+  }
+
+  constructor TwoPhaseGood() {
+    valid := true;
+    new;
+    valid := false;
+    valid := true;
+    foo(this); // no problem, invariant holds by this point
+  }
+
+  constructor TwoPhaseBad() {
+    new;
+    //foo(this); // error
+    valid := true;
+  }
+
+  static method foo(c: C) {
+    assert c.valid by { assert c.invariant(); } // pass
+  }
+}
